completed cond itree proof + simplified parse_pancake def

HOL/panScript.sml
@@ -4,6 +4,7 @@
 
 open panPtreeConversionTheory; (* parse_funs_to_ast *)
 open panSemTheory; (* eval_def *)
+open arithmeticTheory
 
 local
   val f =
@@ -19,7 +20,7 @@ fun parse_pancake q =
   let
     val code = quote_to_strings q |> String.concatWith "\n" |> fromMLstring
   in
-    EVAL “parse_funs_to_ast ^code”
+    rhs $ concl $ SRULE[] $ EVAL “THE (parse_funs_to_ast ^code)”
 end
 
 (* TODO needs to be in panSemTheory *)
@@ -34,57 +35,56 @@ Proof
   Cases_on ‘FLOOKUP s.code fname’ >> rw[]
 QED
 
-(* word related nonsense *)
+(* word nonsense *)
 Theorem load_write_bytearray_thm:
   (∀(b : word8). byte_align b = b) ⇒
   (∀(w : word8). w ∈ s.memaddrs) ⇒
   (∀w. ∃(k : word8). oldmem w = Word k) ⇒
-  mem_load_byte (write_bytearray 0w [v] oldmem s.memaddrs s.be)
-                s.memaddrs s.be 0w
+  mem_load_byte (write_bytearray addr [v] oldmem s.memaddrs s.be)
+                s.memaddrs s.be addr
   = SOME v
 Proof
   rw[mem_load_byte_def] >>
   rw[write_bytearray_def] >>
   rw[mem_store_byte_def] >>
-  first_assum $ qspec_then ‘0w’ strip_assume_tac >>
+  first_assum $ qspec_then ‘addr’ strip_assume_tac >>
   rw[combinTheory.APPLY_UPDATE_THM] >>
   rw[byteTheory.get_byte_set_byte]
 QED
 
-Theorem write_bytearray_preserve_words:
-  (∀w. ∃(k : word8). s.memory w = Word k) ⇒
-  ∀w. ∃(k : word8). (write_bytearray loc l s.memory s.memaddrs s.be) w = Word k
-Proof
-  strip_tac >>
-  qid_spec_tac ‘loc’ >>
-  Induct_on ‘l’ >>
-  rw[write_bytearray_def] >>
-  fs[mem_store_byte_def] >>
-  Cases_on ‘write_bytearray (loc+1w) l s.memory s.memaddrs s.be (byte_align loc)’ >>
-  rw[] >>
-  rw[combinTheory.APPLY_UPDATE_THM] >>
-  Cases_on ‘byte_align loc = w’ >> rw[]
-QED
+(* Theorem write_bytearray_preserve_words: *)
+(*   (∀w. ∃(k : word8). loc ≤ w ∧ w ≤ (loc + LENGTH l) ⇒ s.memory w = Word k) ⇒ *)
+(*   ∀w. ∃(k : word8). (write_bytearray loc l s.memory s.memaddrs s.be) w = Word k *)
+(* Proof *)
+(*   strip_tac >> *)
+(*   qid_spec_tac ‘loc’ >> *)
+(*   Induct_on ‘l’ >> *)
+(*   rw[write_bytearray_def] >> *)
+(*   fs[mem_store_byte_def] >> *)
+(*   Cases_on ‘write_bytearray (loc+1w) l s.memory s.memaddrs s.be (byte_align loc)’ >> *)
+(*   rw[] >> *)
+(*   rw[combinTheory.APPLY_UPDATE_THM] >> *)
+(*   Cases_on ‘byte_align loc = w’ >> rw[] *)
+(* QED *)
 
 (*/
   ffi skip test
  *)
 
-val ffi_ast = rhs $ concl $ parse_pancake ‘
+val ffi_ast = parse_pancake ‘
 fun fn() {
-  #f1(0, 0, 0, 0);
+  #f1(2, 0, 0, 0);
   #f2(0, 0, @base, 1);
   if (ldb @base) == 0 {
-    #f3(0, 0, 0, 0);
+    #f3(3, 0, 0, 0);
   } else {
-    #f4(0, 0, 0, 0);
+    #f4(4, 0, 0, 0);
   }
 }’;
-(* memaddrs *)
 
 Definition ffi_sem_def:
   ffi_sem (s:('a,'ffi) panSem$state) =
-  itree_evaluate (SND $ SND $ HD $ THE ^ffi_ast) s
+  itree_evaluate (SND $ SND $ HD ^ffi_ast) s
 End
 
 (* Inductive walk: *)
@@ -94,82 +94,107 @@ End
 (* [~Ret:] (∀r. walk (Ret r) [] []) *)
 (* End *)
 
+(* TODO simp for future_safe_cases *)
 Inductive next:
   (P (Ret r) ⇒ next P (Ret r)) ∧
   (P (Tau t) ⇒ next P t) ∧
   ((∀a. P (k a)) ⇒ next P (Vis e k))
 End
 
-(* RTC of above AF CTL *)
+(* RTC of above: AF in CTL *)
 Inductive future:
   (P t ⇒ future P t) ∧
   (future P t ⇒ future P (Tau t)) ∧
-  ((∀a. future P (k a)) ⇒ future P (Vis e k))
+  (∀a. future P (k a) ⇒ future P (Vis e k))
 End
 
-Definition the_ffi_def:
-  the_ffi t res f =
-  (∃q. t = (case res of
-              FFI_return new_ffi new_bytes => f new_ffi new_bytes
-            | FFI_final outcome => q outcome))
+(* future but with assumption that bytes written back fit in the passed array *)
+Inductive future_safe:
+  (P t ⇒ future_safe P t) ∧
+  (future_safe P t ⇒ future_safe P (Tau t)) ∧
+  ((∀a outcome new_ffi new_bytes.
+     (a = FFI_final outcome ∨
+      a = FFI_return new_ffi new_bytes ∧ (LENGTH new_bytes ≤ LENGTH array))
+        ⇒ future_safe P (k a))
+   ⇒ future_safe P (Vis (FFI_call s conf array) k))
 End
 
-Theorem write_bytearray_id:
-  (∀(b : word8). byte_align b = b) ⇒
-  (∀(w : word8). w ∈ s.memaddrs) ⇒
-  (∀w. s.memory w = Word (0w : 8 word)) ⇒
-  mem_load_byte (write_bytearray 0w [v]
-                                 (write_bytearray loc l s.memory s.memaddrs s.be)
-                                 s.memaddrs s.be)
-                s.memaddrs s.be 0w
-  = SOME v
+(* TODO why does this simp not work under ctx. no Taus in statements *)
+Theorem future_safe_ignore_tau[simp]:
+  (∀(t' : (α ffi_result, sem_vis_event, 8 result option) itree).
+     ¬P (Tau t')) ⇒ (future_safe P (Tau t) ⇔ future_safe P t)
 Proof
-  metis_tac[write_bytearray_preserve_words, load_write_bytearray_thm]
+  rw[] >>
+  rw[Once future_safe_cases]
 QED
 
-(* TODO simp for future_cases *)
-Theorem ffi_sem_thm:
-  (s.base_addr = 0w) ⇒
-  (∀(b : word8). byte_align b = b) ⇒
-  (∀w. s.memory w = Word (0w : 8 word)) ⇒
-  (∀(w : word8). w ∈ s.memaddrs) ⇒
-  r1 = [0w : 8 word] ⇒
-  future (λt. (∃k k'. k (FFI_return ARB r1) ≈ (Vis (FFI_call "f3" [] []) k') ∧
-                      (t = Vis (FFI_call "f2" [] []) k)) ∨
-              (∃outcome. t = Ret (SOME (FinalFFI outcome))))
-  (ffi_sem s)
+Definition ffi_pred_def:
+  ffi_pred t =
+  ((∃k k' uninit.
+      (t = Vis (FFI_call "f2" [] [uninit]) k) ∧
+      k (FFI_return ARB [1w : 8 word]) ≈ (Vis (FFI_call "f4" [] []) k')) ∨
+   (∃outcome. t = Ret (SOME (FinalFFI outcome))))
+End
+
+Theorem ffi_pred_notau:
+  ¬ffi_pred (Tau (t : (α ffi_result, sem_vis_event, 8 result option) itree))
 Proof
-  qmatch_goalsub_abbrev_tac ‘future P (ffi_sem _)’ >>
+  rw[ffi_pred_def]
+QED
+
+(* byte_align means align (word in bytes) to implicit bit-sized k-word *)
+(* assume all (8-bit) byte-aligned accesses allowed, as in C *)
+(* assume infinite address space *)
+(* assume base memory initially contains some arbitrary word *)
+Theorem ffi_sem_thm:
+  (∀(b : word8). byte_align b = b) ⇒
+  (∀(w : word8). w ∈ s.memaddrs) ⇒
+  (∃uninitb. s.memory s.base_addr = Word uninitb) ⇒
+  future_safe ffi_pred (ffi_sem s)
+Proof
   rw[ffi_sem_def, itree_semantics_def, itree_evaluate_alt] >>
+  assume_tac (GEN_ALL ffi_pred_notau) >>
   (* Seq rw[seq_thm] *)
   rw[itree_mrec_alt, h_prog_def, h_prog_rule_seq_def] >>
   rw[Once itree_iter_thm, Once itree_bind_thm] >>
   (* extcall *)
+  qmatch_goalsub_abbrev_tac
+  ‘bind (h_prog_rule_ext_call «f1» (Const 2w) (Const 0w) (Const 0w) (Const 0w) s)
+   prog’ >>
   rw[itree_mrec_alt, h_prog_def, h_prog_rule_ext_call_def] >>
   rw[miscTheory.read_bytearray_def] >>
+  rw[Once future_safe_cases] >> disj2_tac >>
   (* massaging *)
-  rw[Once future_cases] >> disj2_tac >>
-  rw[Once future_cases] >> disj2_tac >>
-  strip_tac >>
-  (* forall a?, doesn't matter here! *)
-  rw[Once future_cases] >> disj2_tac >>
-  reverse (Cases_on ‘a’) >-
-   (qunabbrev_tac ‘P’ >>
-    rw[Once future_cases] >> disj1_tac) >>
-  rw[Once future_cases] >> disj2_tac >>
+  rpt strip_tac >-
+   (qunabbrev_tac ‘prog’ >>
+    rw[Once future_safe_cases] >>
+    rw[ffi_pred_def]) >>
+  qunabbrev_tac ‘prog’ >> rw[] >>
   (* second seq *)
   rw[itree_mrec_alt, h_prog_def, h_prog_rule_seq_def] >>
   rw[Once itree_iter_thm, Once itree_bind_thm] >>
+  qmatch_goalsub_abbrev_tac ‘bind (h_prog_rule_ext_call _ _ _ _ _ _) kprog’ >>
   (* extcall *)
   rw[itree_mrec_alt, h_prog_def, h_prog_rule_ext_call_def] >>
   rw[miscTheory.read_bytearray_def] >>
-  rw[Once future_cases] >> disj2_tac >>
-  rw[Once future_cases] >> disj1_tac >>
-  qunabbrev_tac ‘P’ >> rw[] >>
+  rw[panSemTheory.write_bytearray_def] >>
+  PURE_REWRITE_TAC[ONE] >> (* wtf *)
+  rw[Once $ cj 2 miscTheory.read_bytearray_def] >>
+  rw[mem_load_byte_def] >>
+  rw[miscTheory.read_bytearray_def] >>
+  (* found tree *)
+  rw[Once future_safe_cases] >> disj1_tac >>
+  rw[ffi_pred_def] >>
+  qunabbrev_tac ‘kprog’ >> rw[] >>
   (* cond *)
   rw[itree_mrec_alt, h_prog_def, h_prog_rule_cond_def] >>
   rw[eval_def, asmTheory.word_cmp_def] >>
-  rw[write_bytearray_id] >>
+  qpat_abbrev_tac ‘stat = (SOME Error, s with <| memory := _; ffi := _ |>)’ >>
+  rw[write_bytearray_def] >>
+  rw[mem_store_byte_def] >>
+  rw[mem_load_byte_def] >>
+  simp[combinTheory.APPLY_UPDATE_THM] >>
+  simp[byteTheory.get_byte_set_byte] >>
   (* third call happens *)
   rw[itree_mrec_alt, h_prog_def, h_prog_rule_ext_call_def] >>
   rw[miscTheory.read_bytearray_def] >>
@@ -180,14 +205,15 @@ QED
    manual loop unrolling isn't too bad with equational rewrites
  *)
 
-(* val loop_ast = rhs $ concl $ parse_pancake ‘ *)
-(* fun fn() { *)
-(*   var x = 1; *)
-(*   x = 0; *)
-(*   while (x < 1) { *)
-(*     x = x + 1; *)
-(*   } *)
-(* }’; *)
+val loop_ast = parse_pancake ‘
+fun fn() {
+  var x = 0;
+  #getnum(0, 0, @base, 1);
+  while (x < (ldb @base)) {
+     #ffi(0, 0, 0, 0);
+     x = x + 1;
+  }
+}’;
 
 (* Definition loop_sem_def: *)
 (*   loop_sem (s:('a,'ffi) panSem$state) = *)
